src/AsyncFS.v
@@ -101,6 +101,7 @@ Module AFS.
   Notation MSLL := BFILE.MSLL.
   Notation MSAllocC := BFILE.MSAllocC.
   Notation MSIAllocC := BFILE.MSIAllocC.
+  Notation MSICache := BFILE.MSICache.
   Notation MSAlloc := BFILE.MSAlloc.
   Import DIRTREE.
 
@@ -128,7 +129,7 @@ Module AFS.
         let^ (mscs, ok) <- LOG.commit (FSXPLog fsxp) mscs;
         If (bool_dec ok true) {
           mscs <- LOG.flushsync (FSXPLog fsxp) mscs;
-          Ret (OK ((BFILE.mk_memstate (MSAlloc ms) mscs (MSAllocC ms) (IAlloc.MSCache ialloc_ms) (MSCache ms)), fsxp))
+          Ret (OK ((BFILE.mk_memstate (MSAlloc ms) mscs (MSAllocC ms) (IAlloc.MSCache ialloc_ms) INODE.IRec.cache0 (MSCache ms)), fsxp))
         } else {
           Ret (Err ELOGOVERFLOW)
         }
@@ -316,9 +317,9 @@ Module AFS.
 
   Definition file_get_attr fsxp inum ams :=
     ms <- LOG.begin (FSXPLog fsxp) (MSLL ams);
-    let^ (ams, attr) <- DIRTREE.getattr fsxp inum (BFILE.mk_memstate (MSAlloc ams) ms (MSAllocC ams) (MSIAllocC ams) (MSCache ams));
+    let^ (ams, attr) <- DIRTREE.getattr fsxp inum (BFILE.mk_memstate (MSAlloc ams) ms (MSAllocC ams) (MSIAllocC ams) (MSICache ams) (MSCache ams));
     ms <- LOG.commit_ro (FSXPLog fsxp) (MSLL ams);
-    Ret ^((BFILE.mk_memstate (MSAlloc ams) ms (MSAllocC ams) (MSIAllocC ams) (MSCache ams)), attr).
+    Ret ^((BFILE.mk_memstate (MSAlloc ams) ms (MSAllocC ams) (MSIAllocC ams) (MSICache ams) (MSCache ams)), attr).
 
   Definition file_get_sz fsxp inum ams :=
     let^ (ams, attr) <- file_get_attr fsxp inum ams;
@@ -326,144 +327,144 @@ Module AFS.
 
   Definition file_set_attr fsxp inum attr ams :=
     ms <- LOG.begin (FSXPLog fsxp) (MSLL ams);
-    ams <- DIRTREE.setattr fsxp inum attr (BFILE.mk_memstate (MSAlloc ams) ms (MSAllocC ams) (MSIAllocC ams) (MSCache ams));
+    ams <- DIRTREE.setattr fsxp inum attr (BFILE.mk_memstate (MSAlloc ams) ms (MSAllocC ams) (MSIAllocC ams) (MSICache ams) (MSCache ams));
     let^ (ms, ok) <- LOG.commit (FSXPLog fsxp) (MSLL ams);
-    Ret ^((BFILE.mk_memstate (MSAlloc ams) ms (MSAllocC ams) (MSIAllocC ams) (MSCache ams)), ok).
+    Ret ^((BFILE.mk_memstate (MSAlloc ams) ms (MSAllocC ams) (MSIAllocC ams) (MSICache ams) (MSCache ams)), ok).
 
   Definition file_set_sz fsxp inum sz ams :=
     ms <- LOG.begin (FSXPLog fsxp) (MSLL ams);
-    ams <- DIRTREE.updattr fsxp inum (INODE.UBytes sz) (BFILE.mk_memstate (MSAlloc ams) ms (MSAllocC ams) (MSIAllocC ams) (MSCache ams));
+    ams <- DIRTREE.updattr fsxp inum (INODE.UBytes sz) (BFILE.mk_memstate (MSAlloc ams) ms (MSAllocC ams) (MSIAllocC ams) (MSICache ams) (MSCache ams));
     let^ (ms, ok) <- LOG.commit (FSXPLog fsxp) (MSLL ams);
-    Ret ^((BFILE.mk_memstate (MSAlloc ams) ms (MSAllocC ams) (MSIAllocC ams) (MSCache ams)), ok).
+    Ret ^((BFILE.mk_memstate (MSAlloc ams) ms (MSAllocC ams) (MSIAllocC ams) (MSICache ams) (MSCache ams)), ok).
 
   Definition read_fblock fsxp inum off ams :=
     ms <- LOG.begin (FSXPLog fsxp) (MSLL ams);
-    let^ (ams, b) <- DIRTREE.read fsxp inum off (BFILE.mk_memstate (MSAlloc ams) ms (MSAllocC ams) (MSIAllocC ams) (MSCache ams));
+    let^ (ams, b) <- DIRTREE.read fsxp inum off (BFILE.mk_memstate (MSAlloc ams) ms (MSAllocC ams) (MSIAllocC ams) (MSICache ams) (MSCache ams));
     ms <- LOG.commit_ro (FSXPLog fsxp) (MSLL ams);
-    Ret ^((BFILE.mk_memstate (MSAlloc ams) ms (MSAllocC ams) (MSIAllocC ams) (MSCache ams)), b).
+    Ret ^((BFILE.mk_memstate (MSAlloc ams) ms (MSAllocC ams) (MSIAllocC ams) (MSICache ams) (MSCache ams)), b).
 
   Definition file_truncate fsxp inum sz ams :=
     ms <- LOG.begin (FSXPLog fsxp) (MSLL ams);
-    let^ (ams, ok) <- DIRTREE.truncate fsxp inum sz (BFILE.mk_memstate (MSAlloc ams) ms (MSAllocC ams) (MSIAllocC ams) (MSCache ams));
+    let^ (ams, ok) <- DIRTREE.truncate fsxp inum sz (BFILE.mk_memstate (MSAlloc ams) ms (MSAllocC ams) (MSIAllocC ams) (MSICache ams) (MSCache ams));
     match ok with
     | Err e =>
       ms <- LOG.abort (FSXPLog fsxp) (MSLL ams);
-      Ret ^((BFILE.mk_memstate (MSAlloc ams) ms (MSAllocC ams) (MSIAllocC ams) (MSCache ams)), Err e)
+      Ret ^((BFILE.mk_memstate (MSAlloc ams) ms (MSAllocC ams) (MSIAllocC ams) (MSICache ams) (MSCache ams)), Err e)
     | OK _ =>
       let^ (ms, ok) <- LOG.commit (FSXPLog fsxp) (MSLL ams);
       If (bool_dec ok true) {
-        Ret ^((BFILE.mk_memstate (MSAlloc ams) ms (MSAllocC ams) (MSIAllocC ams) (MSCache ams)), OK tt)
+        Ret ^((BFILE.mk_memstate (MSAlloc ams) ms (MSAllocC ams) (MSIAllocC ams) (MSICache ams) (MSCache ams)), OK tt)
       } else {
-        Ret ^((BFILE.mk_memstate (MSAlloc ams) ms (MSAllocC ams) (MSIAllocC ams) (MSCache ams)), Err ELOGOVERFLOW)
+        Ret ^((BFILE.mk_memstate (MSAlloc ams) ms (MSAllocC ams) (MSIAllocC ams) (MSICache ams) (MSCache ams)), Err ELOGOVERFLOW)
       }
     end.
 
   (* update an existing block directly.  XXX dwrite happens to sync metadata. *)
   Definition update_fblock_d fsxp inum off v ams :=
     ms <- LOG.begin (FSXPLog fsxp) (MSLL ams);
-    ams <- DIRTREE.dwrite fsxp inum off v (BFILE.mk_memstate (MSAlloc ams) ms (MSAllocC ams) (MSIAllocC ams) (MSCache ams));
+    ams <- DIRTREE.dwrite fsxp inum off v (BFILE.mk_memstate (MSAlloc ams) ms (MSAllocC ams) (MSIAllocC ams) (MSICache ams) (MSCache ams));
     ms <- LOG.commit_ro (FSXPLog fsxp) (MSLL ams);
-    Ret ^((BFILE.mk_memstate (MSAlloc ams) ms (MSAllocC ams) (MSIAllocC ams) (MSCache ams))).
+    Ret ^((BFILE.mk_memstate (MSAlloc ams) ms (MSAllocC ams) (MSIAllocC ams) (MSICache ams) (MSCache ams))).
 
   Definition update_fblock fsxp inum off v ams :=
     ms <- LOG.begin (FSXPLog fsxp) (MSLL ams);
-    ams <- DIRTREE.write fsxp inum off v (BFILE.mk_memstate (MSAlloc ams) ms (MSAllocC ams) (MSIAllocC ams) (MSCache ams));
+    ams <- DIRTREE.write fsxp inum off v (BFILE.mk_memstate (MSAlloc ams) ms (MSAllocC ams) (MSIAllocC ams) (MSICache ams) (MSCache ams));
     let^ (ms, ok) <- LOG.commit (FSXPLog fsxp) (MSLL ams);
-    Ret ^((BFILE.mk_memstate (MSAlloc ams) ms (MSAllocC ams) (MSIAllocC ams) (MSCache ams)), ok).
+    Ret ^((BFILE.mk_memstate (MSAlloc ams) ms (MSAllocC ams) (MSIAllocC ams) (MSICache ams) (MSCache ams)), ok).
 
   (* sync only data blocks of a file. *)
   Definition file_sync fsxp inum ams :=
     ms <- LOG.begin (FSXPLog fsxp) (MSLL ams);
-    ams <- DIRTREE.datasync fsxp inum (BFILE.mk_memstate (MSAlloc ams) ms (MSAllocC ams) (MSIAllocC ams) (MSCache ams));
+    ams <- DIRTREE.datasync fsxp inum (BFILE.mk_memstate (MSAlloc ams) ms (MSAllocC ams) (MSIAllocC ams) (MSICache ams) (MSCache ams));
     ms <- LOG.commit_ro (FSXPLog fsxp) (MSLL ams);
-    Ret ^((BFILE.mk_memstate (MSAlloc ams) ms (MSAllocC ams) (MSIAllocC ams) (MSCache ams))).
+    Ret ^((BFILE.mk_memstate (MSAlloc ams) ms (MSAllocC ams) (MSIAllocC ams) (MSICache ams) (MSCache ams))).
 
   Definition readdir fsxp dnum ams :=
     ms <- LOG.begin (FSXPLog fsxp) (MSLL ams);
-    let^ (ams, files) <- SDIR.readdir (FSXPLog fsxp) (FSXPInode fsxp) dnum (BFILE.mk_memstate (MSAlloc ams) ms (MSAllocC ams) (MSIAllocC ams) (MSCache ams));
+    let^ (ams, files) <- SDIR.readdir (FSXPLog fsxp) (FSXPInode fsxp) dnum (BFILE.mk_memstate (MSAlloc ams) ms (MSAllocC ams) (MSIAllocC ams) (MSICache ams) (MSCache ams));
     ms <- LOG.commit_ro (FSXPLog fsxp) (MSLL ams);
-    Ret ^((BFILE.mk_memstate (MSAlloc ams) ms (MSAllocC ams) (MSIAllocC ams) (MSCache ams)), files).
+    Ret ^((BFILE.mk_memstate (MSAlloc ams) ms (MSAllocC ams) (MSIAllocC ams) (MSICache ams) (MSCache ams)), files).
 
   Definition create fsxp dnum name ams :=
     ms <- LOG.begin (FSXPLog fsxp) (MSLL ams);
-    let^ (ams, oi) <- DIRTREE.mkfile fsxp dnum name (BFILE.mk_memstate (MSAlloc ams) ms (MSAllocC ams) (MSIAllocC ams) (MSCache ams));
+    let^ (ams, oi) <- DIRTREE.mkfile fsxp dnum name (BFILE.mk_memstate (MSAlloc ams) ms (MSAllocC ams) (MSIAllocC ams) (MSICache ams) (MSCache ams));
     match oi with
       | Err e =>
         ms <- LOG.abort (FSXPLog fsxp) (MSLL ams);
-          Ret ^((BFILE.mk_memstate (MSAlloc ams) ms (MSAllocC ams) (MSIAllocC ams) (MSCache ams)), Err e)
+          Ret ^((BFILE.mk_memstate (MSAlloc ams) ms (MSAllocC ams) (MSIAllocC ams) (MSICache ams) (MSCache ams)), Err e)
       | OK inum =>
         let^ (ms, ok) <- LOG.commit (FSXPLog fsxp) (MSLL ams);
         match ok with
-          | true => Ret ^((BFILE.mk_memstate (MSAlloc ams) ms (MSAllocC ams) (MSIAllocC ams) (MSCache ams)), OK inum)
-          | false => Ret ^((BFILE.mk_memstate (MSAlloc ams) ms (MSAllocC ams) (MSIAllocC ams) (MSCache ams)), Err ELOGOVERFLOW)
+          | true => Ret ^((BFILE.mk_memstate (MSAlloc ams) ms (MSAllocC ams) (MSIAllocC ams) (MSICache ams) (MSCache ams)), OK inum)
+          | false => Ret ^((BFILE.mk_memstate (MSAlloc ams) ms (MSAllocC ams) (MSIAllocC ams) (MSICache ams) (MSCache ams)), Err ELOGOVERFLOW)
         end
     end.
 
   Definition mksock fsxp dnum name ams :=
     ms <- LOG.begin (FSXPLog fsxp) (MSLL ams);
-    let^ (ams, oi) <- DIRTREE.mkfile fsxp dnum name (BFILE.mk_memstate (MSAlloc ams) ms (MSAllocC ams) (MSIAllocC ams) (MSCache ams));
+    let^ (ams, oi) <- DIRTREE.mkfile fsxp dnum name (BFILE.mk_memstate (MSAlloc ams) ms (MSAllocC ams) (MSIAllocC ams) (MSICache ams) (MSCache ams));
     match oi with
       | Err e =>
         ms <- LOG.abort (FSXPLog fsxp) (MSLL ams);
-        Ret ^((BFILE.mk_memstate (MSAlloc ams) ms (MSAllocC ams) (MSIAllocC ams) (MSCache ams)), Err e)
+        Ret ^((BFILE.mk_memstate (MSAlloc ams) ms (MSAllocC ams) (MSIAllocC ams) (MSICache ams) (MSCache ams)), Err e)
       | OK inum =>
         ams <- BFILE.updattr (FSXPLog fsxp) (FSXPInode fsxp) inum (INODE.UType $1) ams;
         let^ (ms, ok) <- LOG.commit (FSXPLog fsxp) (MSLL ams);
         match ok with
-          | true => Ret ^((BFILE.mk_memstate (MSAlloc ams) ms (MSAllocC ams) (MSIAllocC ams) (MSCache ams)), OK inum)
-          | false => Ret ^((BFILE.mk_memstate (MSAlloc ams) ms (MSAllocC ams) (MSIAllocC ams) (MSCache ams)), Err ELOGOVERFLOW)
+          | true => Ret ^((BFILE.mk_memstate (MSAlloc ams) ms (MSAllocC ams) (MSIAllocC ams) (MSICache ams) (MSCache ams)), OK inum)
+          | false => Ret ^((BFILE.mk_memstate (MSAlloc ams) ms (MSAllocC ams) (MSIAllocC ams) (MSICache ams) (MSCache ams)), Err ELOGOVERFLOW)
         end
     end.
 
   Definition mkdir fsxp dnum name ams :=
     ms <- LOG.begin (FSXPLog fsxp) (MSLL ams);
-    let^ (ams, oi) <- DIRTREE.mkdir fsxp dnum name (BFILE.mk_memstate (MSAlloc ams) ms (MSAllocC ams) (MSIAllocC ams) (MSCache ams));
+    let^ (ams, oi) <- DIRTREE.mkdir fsxp dnum name (BFILE.mk_memstate (MSAlloc ams) ms (MSAllocC ams) (MSIAllocC ams) (MSICache ams) (MSCache ams));
     match oi with
       | Err e =>
         ms <- LOG.abort (FSXPLog fsxp) (MSLL ams);
-          Ret ^((BFILE.mk_memstate (MSAlloc ams) ms (MSAllocC ams) (MSIAllocC ams) (MSCache ams)), Err e)
+          Ret ^((BFILE.mk_memstate (MSAlloc ams) ms (MSAllocC ams) (MSIAllocC ams) (MSICache ams) (MSCache ams)), Err e)
       | OK inum =>
         let^ (ms, ok) <- LOG.commit (FSXPLog fsxp) (MSLL ams);
         match ok with
-          | true => Ret ^((BFILE.mk_memstate (MSAlloc ams) ms (MSAllocC ams) (MSIAllocC ams) (MSCache ams)), OK inum)
-          | false => Ret ^((BFILE.mk_memstate (MSAlloc ams) ms (MSAllocC ams) (MSIAllocC ams) (MSCache ams)), Err ELOGOVERFLOW)
+          | true => Ret ^((BFILE.mk_memstate (MSAlloc ams) ms (MSAllocC ams) (MSIAllocC ams) (MSICache ams) (MSCache ams)), OK inum)
+          | false => Ret ^((BFILE.mk_memstate (MSAlloc ams) ms (MSAllocC ams) (MSIAllocC ams) (MSICache ams) (MSCache ams)), Err ELOGOVERFLOW)
         end
     end.
 
   Definition delete fsxp dnum name ams :=
     ms <- LOG.begin (FSXPLog fsxp) (MSLL ams);
-    let^ (ams, ok) <- DIRTREE.delete fsxp dnum name (BFILE.mk_memstate (MSAlloc ams) ms (MSAllocC ams) (MSIAllocC ams) (MSCache ams));
+    let^ (ams, ok) <- DIRTREE.delete fsxp dnum name (BFILE.mk_memstate (MSAlloc ams) ms (MSAllocC ams) (MSIAllocC ams) (MSICache ams) (MSCache ams));
     match ok with
     | OK _ =>
        let^ (ms, ok) <- LOG.commit (FSXPLog fsxp) (MSLL ams);
        match ok with
-       | true => Ret ^((BFILE.mk_memstate (MSAlloc ams) ms (MSAllocC ams) (MSIAllocC ams) (MSCache ams)), OK tt)
-       | false => Ret ^((BFILE.mk_memstate (MSAlloc ams) ms (MSAllocC ams) (MSIAllocC ams) (MSCache ams)), Err ELOGOVERFLOW)
+       | true => Ret ^((BFILE.mk_memstate (MSAlloc ams) ms (MSAllocC ams) (MSIAllocC ams) (MSICache ams) (MSCache ams)), OK tt)
+       | false => Ret ^((BFILE.mk_memstate (MSAlloc ams) ms (MSAllocC ams) (MSIAllocC ams) (MSICache ams) (MSCache ams)), Err ELOGOVERFLOW)
        end
     | Err e =>
       ms <- LOG.abort (FSXPLog fsxp) (MSLL ams);
-      Ret ^((BFILE.mk_memstate (MSAlloc ams) ms (MSAllocC ams) (MSIAllocC ams) (MSCache ams)), Err e)
+      Ret ^((BFILE.mk_memstate (MSAlloc ams) ms (MSAllocC ams) (MSIAllocC ams) (MSICache ams) (MSCache ams)), Err e)
     end.
 
   Definition lookup fsxp dnum names ams :=
     ms <- LOG.begin (FSXPLog fsxp) (MSLL ams);
-    let^ (ams, r) <- DIRTREE.namei fsxp dnum names (BFILE.mk_memstate (MSAlloc ams) ms (MSAllocC ams) (MSIAllocC ams) (MSCache ams));
+    let^ (ams, r) <- DIRTREE.namei fsxp dnum names (BFILE.mk_memstate (MSAlloc ams) ms (MSAllocC ams) (MSIAllocC ams) (MSICache ams) (MSCache ams));
     ms <- LOG.commit_ro (FSXPLog fsxp) (MSLL ams);
-    Ret ^((BFILE.mk_memstate (MSAlloc ams) ms (MSAllocC ams) (MSIAllocC ams) (MSCache ams)), r).
+    Ret ^((BFILE.mk_memstate (MSAlloc ams) ms (MSAllocC ams) (MSIAllocC ams) (MSICache ams) (MSCache ams)), r).
 
   Definition rename fsxp dnum srcpath srcname dstpath dstname ams :=
     ms <- LOG.begin (FSXPLog fsxp) (MSLL ams);
-    let^ (ams, r) <- DIRTREE.rename fsxp dnum srcpath srcname dstpath dstname (BFILE.mk_memstate (MSAlloc ams) ms (MSAllocC ams) (MSIAllocC ams) (MSCache ams));
+    let^ (ams, r) <- DIRTREE.rename fsxp dnum srcpath srcname dstpath dstname (BFILE.mk_memstate (MSAlloc ams) ms (MSAllocC ams) (MSIAllocC ams) (MSICache ams) (MSCache ams));
     match r with
     | OK _ =>
       let^ (ms, ok) <- LOG.commit (FSXPLog fsxp) (MSLL ams);
       match ok with
-      | true => Ret ^((BFILE.mk_memstate (MSAlloc ams) ms (MSAllocC ams) (MSIAllocC ams) (MSCache ams)), OK tt)
-      | false => Ret ^((BFILE.mk_memstate (MSAlloc ams) ms (MSAllocC ams) (MSIAllocC ams) (MSCache ams)), Err ELOGOVERFLOW)
+      | true => Ret ^((BFILE.mk_memstate (MSAlloc ams) ms (MSAllocC ams) (MSIAllocC ams) (MSICache ams) (MSCache ams)), OK tt)
+      | false => Ret ^((BFILE.mk_memstate (MSAlloc ams) ms (MSAllocC ams) (MSIAllocC ams) (MSICache ams) (MSCache ams)), Err ELOGOVERFLOW)
       end
     | Err e =>
       ms <- LOG.abort (FSXPLog fsxp) (MSLL ams);
-      Ret ^((BFILE.mk_memstate (MSAlloc ams) ms (MSAllocC ams) (MSIAllocC ams) (MSCache ams)), Err e)
+      Ret ^((BFILE.mk_memstate (MSAlloc ams) ms (MSAllocC ams) (MSIAllocC ams) (MSICache ams) (MSCache ams)), Err e)
     end.
 
   (* sync directory tree; will flush all outstanding changes to tree (but not dupdates to files) *)
@@ -478,7 +479,7 @@ Module AFS.
   Definition umount fsxp ams :=
     ams <- DIRTREE.sync fsxp ams;
     ms <- LOG.sync_cache (FSXPLog fsxp) (MSLL ams);
-    Ret ^((BFILE.mk_memstate (MSAlloc ams) ms (MSAllocC ams) (MSIAllocC ams) (MSCache ams))).
+    Ret ^((BFILE.mk_memstate (MSAlloc ams) ms (MSAllocC ams) (MSIAllocC ams) (MSICache ams) (MSCache ams))).
 
   Definition statfs fsxp ams :=
     ms <- LOG.begin (FSXPLog fsxp) (MSLL ams);
@@ -488,7 +489,7 @@ Module AFS.
      *)
     ms <- LOG.commit_ro (FSXPLog fsxp) ms;
     (* Ret ^(mscs, free_blocks, free_inodes).  *)
-    Ret ^((BFILE.mk_memstate (MSAlloc ams) ms (MSAllocC ams) (MSIAllocC ams) (MSCache ams)), 0, 0).
+    Ret ^((BFILE.mk_memstate (MSAlloc ams) ms (MSAllocC ams) (MSIAllocC ams) (MSICache ams) (MSCache ams)), 0, 0).
 
   (* Recover theorems *)
 
