src/DirCache.v
@@ -93,7 +93,7 @@ Module CacheOneDir.
 
   Definition rep_macro Fi Fm m bxp ixp (inum : addr) dsmap ilist frees f ms : @pred _ addr_eq_dec valuset :=
     (exists flist,
-     [[[ m ::: Fm * BFILE.rep bxp ixp flist ilist frees (BFILE.MSAllocC ms) (BFILE.MSCache ms) ]]] *
+     [[[ m ::: Fm * BFILE.rep bxp ixp flist ilist frees (BFILE.MSAllocC ms) (BFILE.MSCache ms) (BFILE.MSICache ms) ]]] *
      [[[ flist ::: Fi * inum |-> f ]]] *
      [[ rep f dsmap ]] )%pred.
 
